subj red and prog complete

src/session.v
@@ -9,19 +9,22 @@ src.part src.gttreeh src.step src.merge src.projection src.lcontext src.wfltt.
 
 Inductive session: Type :=
   | s_ind : part   -> process -> session
-  | s_par : session -> session -> session.
+  | s_par : session -> session -> session
+  | s_zero : session.
   
 Notation "p '<--' P"   :=  (s_ind p P) (at level 50, no associativity).
 Notation "s1 '|||' s2" :=  (s_par s1 s2) (at level 50, no associativity).
 
 Inductive ForallT (P : part -> process -> Prop) : session -> Prop := 
   | ForallT_mono : forall pt op, P pt op -> ForallT P (pt <-- op)
-  | ForallT_par : forall (M1 M2 : session), ForallT P M1 -> ForallT P M2 -> ForallT P (M1 ||| M2). 
-  
+  | ForallT_par : forall (M1 M2 : session), ForallT P M1 -> ForallT P M2 -> ForallT P (M1 ||| M2)
+  | ForallT_zero: ForallT P s_zero.
+
 Fixpoint flattenT (M : session) : (list part) := 
   match M with 
     | p <-- _   => p :: nil
     | M1 ||| M2 => flattenT M1 ++ flattenT M2
+    | s_zero => nil
   end.
 
 Definition InT (pt : part) (M : session) : Prop :=
@@ -30,15 +33,15 @@ Definition InT (pt : part) (M : session) : Prop :=
 Definition in_not_end (pt:part) (gamma: tctx) := exists x, M.find pt gamma=Some x /\ x <> ltt_end.  
 
 Inductive unfoldP : relation session := 
-  | pc_sub   : forall p P Q M, substitutionP 0 0 0 (p_rec P) P Q -> unfoldP (p <-- (p_rec P) ||| M) (p <-- Q ||| M)
-  | pc_subm  : forall p P Q, substitutionP 0 0 0 (p_rec P) P Q -> unfoldP (p <-- (p_rec P)) (p <-- Q)
+  | pc_tau   : forall p P Q M, tauP P Q -> unfoldP ((p <-- P) ||| M) ((p <-- Q) ||| M)
   | pc_refl  : forall M, unfoldP M M
   | pc_trans : forall M M' M'', unfoldP M M' -> unfoldP M' M'' -> unfoldP M M''
   | pc_par1  : forall M M', unfoldP (M ||| M') (M' ||| M)
   | pc_par2  : forall M M' M'', unfoldP ((M ||| M') ||| M'') (M ||| (M' ||| M''))
   | pc_par1m : forall M M' M'', unfoldP ((M ||| M') ||| M'') ((M' ||| M) ||| M'')
-  | pc_par2m : forall M M' M'' M''', unfoldP (((M ||| M') ||| M'') ||| M''') ((M ||| (M' ||| M'')) ||| M''').
-
+  | pc_par2m : forall M M' M'' M''', unfoldP (((M ||| M') ||| M'') ||| M''') ((M ||| (M' ||| M'')) ||| M''')
+  | pc_zero_elim : forall M, unfoldP (M ||| s_zero) M
+  | pc_zero_intro : forall M, unfoldP  M (M ||| s_zero).
 
 Inductive typ_sess : session -> tctx -> Prop := 
   | t_sess : forall M gamma (Hassocable: exists g, wfgC g /\ assoc gamma g), tctx_wf gamma ->
@@ -52,23 +55,7 @@ Inductive betaP: relation session :=
   | r_comm  : forall p q xs y l e v Q M, 
               onth l xs = Some y -> stepE e (e_val v) -> 
               betaP ((p <-- (p_recv q xs)) ||| (q <-- (p_send p l e Q)) ||| M)
-                    ((p <-- subst_expr_proc y (e_val v) 0 0) ||| (q <-- Q) ||| M)
-  | rt_ite  : forall p e P Q M,
-              stepE e (e_val (vbool true)) ->
-              betaP ((p <-- (p_ite e P Q)) ||| M) ((p <-- P) ||| M)
-  | rf_ite  : forall p e P Q M,
-              stepE e (e_val (vbool false)) ->
-              betaP ((p <-- (p_ite e P Q)) ||| M) ((p <-- Q) ||| M)
-  | r_commu  : forall p q xs y l e v Q, 
-              onth l xs = Some y -> stepE e (e_val v) -> 
-              betaP ((p <-- (p_recv q xs)) ||| (q <-- (p_send p l e Q)))
-                    ((p <-- subst_expr_proc y (e_val v) 0 0) ||| (q <-- Q))
-  | rt_iteu  : forall p e P Q,
-              stepE e (e_val (vbool true)) ->
-              betaP ((p <-- (p_ite e P Q))) ((p <-- P))
-  | rf_iteu  : forall p e P Q,
-              stepE e (e_val (vbool false)) ->
-              betaP ((p <-- (p_ite e P Q))) ((p <-- Q))
+                    ((p <-- subst_expr_proc y (e_val v) 0 0) ||| (q <-- Q) ||| M) 
   | r_struct: forall M1 M1' M2 M2', unfoldP M1 M1' -> unfoldP M2' M2 -> betaP M1' M2' -> betaP M1 M2.
 
 Definition beta_multistep := multi betaP.
