lemma/main.v
@@ -8,6 +8,10 @@ From SST Require Import src.header src.sim src.expr src.process src.local
 src.global src.balanced src.typecheck src.part src.gttreeh src.path_props src.step src.merge src.projection src.session src.lcontext.  
 From SST Require Import lemma.inversion lemma.inversion_expr lemma.completeness lemma.substitution_helper lemma.substitution lemma.decidable_helper lemma.decidable lemma.expr lemma.part lemma.step 
 lemma.projection_helper lemma.projection lemma.main_helper lemma.soundness lemma.liveness_helpers. 
+
+
+Search substitutionP guardP.
+
 Lemma active_parts_subset: forall gamma pt p q ell gamma', 
     tctxR gamma (lcomm p q ell) gamma' -> in_not_end pt gamma' -> in_not_end pt gamma.
     Proof.
@@ -186,157 +190,7 @@ Proof.
     }
     eapply typ_after_step_not_in_label with (gamma:=gamma);try exact Hstep;try easy.
   }
-  {
-    inversion Hsess;subst;inversion H3;subst. inversion H6;subst;destr_hyps.
-    eapply inv_proc_ite in H8 as Hinvpr;try reflexivity;destr_hyps.
-    exists gamma;split;try solve [constructor 2]. 
-    rename P into Pp, Q into Qp.
-    constructor;try easy. exists x0;tauto.
-    constructor;try easy. constructor. exists x;split;try easy;split. eapply tc_sub;try exact H11;try easy.
-    eapply typable_implies_wfC in H8;try easy.
-    intros. 
-    specialize (H9 n). destr_hyps. inversion H9;subst. exists 0. constructor.
-    exists m. easy. 
-  }
-  {
-   inversion Hsess;subst;inversion H3;subst. inversion H6;subst;destr_hyps.
-    eapply inv_proc_ite in H8 as Hinvpr;try reflexivity;destr_hyps.
-    exists gamma;split;try solve [constructor 2]. 
-    rename P into Pp, Q into Qp.
-    constructor;try easy. exists x0;tauto.
-    constructor;try easy. constructor. exists x;split;try easy;split. eapply tc_sub;try exact H12;try easy.
-    eapply typable_implies_wfC in H8;try easy.
-    intros. 
-    specialize (H9 n). destr_hyps. inversion H9;subst. exists 0. constructor.
-    exists m. easy.  
-  }
-  {
-     inversion Hsess;subst. rename H1 into Htwf, H2 into Hins, H3 into Hnodup, H4 into Hfat.
-    inversion Hfat;subst. inversion H3;subst. inversion H4;subst. 
-    
-    destruct H2 as [Tp [Htp [Htypp Hguardp]]]. destruct H5 as [Tq [Htq [Htypq Hguardq]]].
-    eapply inv_proc_recv in Htypp as Hrec_inv;try reflexivity.
-    eapply inv_proc_send in Htypq as Hsend_inv;try reflexivity.
-    destr_hyps.
-    rename x2 into g.
-    eapply assoc.subtype_recv_inv1 in H8 as Hn;destr_hyps;subst.
-    eapply assoc.subtype_send_inv1 in H7 as Hn;destr_hyps;subst.
-    rename H11 into Hassoc, H5 into Hwfg.
-    assert(Hispartsp : isgPartsC p g).
-    {
-      destruct (decidable_isgPartsC g p);try easy.
-      specialize (Hassoc p). destruct Hassoc.
-      specialize (H12 H5 _ Htp);easy. 
-    }
-    assert(Hispartsq : isgPartsC q g).
-    {
-      destruct (decidable_isgPartsC g q);try easy.
-      specialize (Hassoc q). destruct Hassoc.
-      specialize (H12 H5 _ Htq);easy. 
-    }
-    eapply subtype_recv_inv in H8 as Hsinvrec.
-    eapply subtype_send_inv in H7 as Hsinvsend.
 
-    assert (Honthl : onth l (extendLis l (Some (x, x0))) = Some (x,x0)) by
-    eapply extendExtract.
-    eapply Forall2R_prop in Hsinvsend;try exact Honthl;tac_sanitize.
-    assert(Hpq: p <>q).
-    {
-      red;intros;subst;congruence. 
-    }
-    assert (Hsubp: assoc.issubProj (ltt_send p x3) g q).
-    {
-      tac_use_assoc Hassoc q Hispartsq;destr_hyps. 
-      rewrite Htq in H5; inversion H5;subst;easy.
-    }
-    assert (Hsubq: assoc.issubProj (ltt_recv q x2) g p).
-    {
-      tac_use_assoc Hassoc p Hispartsp;destr_hyps. 
-      rewrite Htp in H5;inversion H5;subst;easy.
-    }
-    eapply assoc.lem_6_16_simul_subproj with (q:=p) (xp:=x3) (xq:=x2) 
-    in Hispartsq as Hsim;try easy;try solve [tac_wfl_to_slist
-
-    | 
-    specialize (Htwf _ _ Htq); pinversion Htwf; subst;try apply wfltt.wfltt_mon;try easy
-    |
-    
-    specialize (Htwf _ _ Htp); pinversion Htwf; subst;try apply wfltt.wfltt_mon
-    ;try easy
-    ].
-    eapply Forall2R_prop in Hsim;try exact H12;tac_sanitize.
-    eapply simple_red_comm in Htp as Hstep;try exact Htq;try easy;
-    try exact H12;try exact H15;try easy.
-    set (gamma' := (M.add q x4 (M.add p x10 (M.remove q (M.remove p gamma))))).
-    exists gamma'.
-    split;try solve [constructor;red;exists q, p, l;try easy].
-    constructor;try easy.
-    assert(Hprojable: projectableA g) by (eapply assoc_implies_projectable in Hassoc;try easy).
-    eapply assoc_completeness with (g:=g) in Hstep as Hgstep;try easy. 
-    destr_hyps. exists x;split;try easy. eapply wfgC_after_step in H11;try easy.
-    
-    eapply wfltt.tctx_wf_after_red_comm;try exact Htwf;try exact Hstep.
-    
-    intros.
-    eapply active_parts_subset in H5;try exact Hstep.
-    specialize (Hins _ H5) as Hins'.
-    red in Hins';simpl in Hins'.
-    red;simpl. easy.
-    repeat constructor.
-    rename x10 into Tp', x4 into Tq'.
-    {
-      exists Tp'.
-      split;unfold gamma';try autorewrite with mmaps;try easy.
-      split. 
-      eapply Forall2_prop_r in H9;try exact H;tac_sanitize.
-      eapply Forall2R_prop in Hsinvrec;try exact H15;tac_sanitize.
-      rewrite H11 in H18;inversion H18;subst;clear H18.
-      eapply _subst_expr_var with (S:=x11);try easy.
-      eapply tc_sub;try exact H20;try easy.
-
-      eapply wfC_recv with (q:=q); try exact H15.
-      eapply typable_implies_wfC;try exact Htypp.
-      
-      + eapply sc_sub;try exact H19. eapply sc_sub;try exact H16;
-      eapply sc_sub with (s:=x5);try easy. eapply expr_typ_step;try exact H1;try easy.
-      eapply guardP_subst_expr;try easy.
-      
-      + eapply guardP_cont_recv_n; try exact H;try easy.
-    }
-    {
-      unfold gamma';autorewrite with mmaps.
-      exists x4. repeat split;try easy. eapply tc_sub;try exact H6;try easy.
-      eapply wfC_send with (p:=p); try exact H12.
-      eapply typable_implies_wfC;try exact Htypq.
-
-      intros.  specialize (Hguardq (S n)) as Hq'. destr_hyps. inversion H5;subst.
-      exists x. easy.
-    }
-  }
-  {
-    inversion Hsess;subst;inversion H3;subst. destr_hyps.
-    eapply inv_proc_ite in H6 as Hinvpr;try reflexivity;destr_hyps.
-    exists gamma;split;try solve [constructor 2]. 
-    rename P into Pp, Q into Qp.
-    constructor;try easy. exists x0;tauto.
-    constructor;try easy.  exists x;split;try easy;split. eapply tc_sub;try exact H11;try easy.
-    eapply typable_implies_wfC in H6;try easy.
-    intros. 
-    specialize (H7 n). destr_hyps. inversion H7;subst. exists 0. constructor.
-    exists m. easy. 
-  }
-  {
-    inversion Hsess;subst;inversion H3;subst. destr_hyps.
-    eapply inv_proc_ite in H6 as Hinvpr;try reflexivity;destr_hyps.
-    exists gamma;split;try solve [constructor 2]. 
-    rename P into Pp, Q into Qp.
-    constructor;try easy. exists x0;tauto.
-    constructor;try easy.  exists x;split;try easy;split. eapply tc_sub;try exact H10;try easy.
-    eapply typable_implies_wfC in H6;try easy.
-    intros. 
-    specialize (H7 n). destr_hyps. inversion H7;subst. exists 0. constructor.
-    exists m. easy. 
-  }
   {
     eapply typ_after_unfold in Hsess as Hunfold1;try exact H.
     eapply IHHbeta in Hunfold1 as Hu2. destr_hyps. eapply typ_after_unfold in H1;try exact H0.
@@ -386,53 +240,6 @@ Hint Constructors unfoldP :procs.
 Search unfoldP.
 Hint Resolve unf_cont_r unf_cont_l betaPr_unfold_h betaPr_unfold:procs.
 Print HintDb procs.
-Lemma ForallT_or_all_or_some P Q: forall M,  
-ForallT (fun u v => P u v \/ Q u v) M -> ForallT (fun u v => P u v) M \/ 
-(exists M' p T, unfoldP M ((p <-- T) |||M') /\ Q p T) \/ 
-(exists p T, unfoldP M ((p <-- T)) /\ Q p T)
-.
-Proof.
-  induction M.
-  {
-    intros. inversion H;subst. destruct H1. left. constructor. easy.
-
-    right. right. exists n, p.  split. constructor. tauto. 
-  }
-  {
-    intros * HPvQ.
-    inversion HPvQ;subst.
-    specialize (IHM1 H1).
-    specialize (IHM2 H2).
-    destruct (IHM1).
-    {
-      destruct (IHM2).
-      left. constructor;easy. 
-      right. destruct H0.
-      {
-         destruct H0 as [M' [p [T Hpt]]]. left. exists (M1 ||| M'), p, T.
-         split;try tauto.
-        
-        destruct Hpt.
-        
-        eapply unf_cont_r with (M1:=M1) in H0.
-
-        eauto with procs.
-      } 
-      {
-       destruct H0 as [p [T Hpt]]. left. exists  M1, p, T.
-       split;try tauto. destr_hyps.
-       eauto with procs.
-      }
-    }
-    destruct H.
-	{
-		destr_hyps. right. left. exists (x|||M2), x0, x1. split;try eauto with procs.
-	}
-	{
-		destr_hyps. right. left. exists ( M2), x, x0. eauto with procs.  	
-	}
-  }
-Qed.
 
   
 Theorem prog : forall M G, typ_sess M G -> (exists M', unfoldP M M' /\ (ForallT (fun _ P => P = p_inact) M')) \/ exists M', betaP M M'.
@@ -445,41 +252,9 @@ Proof.
 	eapply assoc_implies_end_or_atleast_send in Hassoc as Hdil;try easy.
 	destruct Hdil as [Hdil | Hdil].
 	{
-		eapply canonical_glob_n in Hdil;try exact Hsess.
+		eapply canonical_glob_n_strong in Hdil;try exact Hsess.
 		destruct Hdil as [M' [Hunf Hfat]]. 
-		eapply ForallT_or_all_or_some in Hfat. destruct Hfat. left; exists M'. split;tauto.
-		
-		destruct H. 
-		+ destr_hyps;subst.
-		assert(exists M2, betaP (x0 <-- (p_ite x2 x3 x4) ||| x) M2).
-		{
-		eapply inv_proc_ite in H1;try reflexivity;destr_hyps.
-		Search sbool.
-		eapply expr_eval_b in H4.
-		destruct H4.
-		eapply rt_ite with (p:=x0) (P:=x3) (Q:=x4) (M:=x) in H4; exists ((x0 <-- x3) ||| x); easy.      
-		eapply rf_ite with (p:=x0) (P:=x3) (Q:=x4) (M:=x) in H4; exists ((x0 <-- x4) ||| x); easy.
-		}
-		destr_hyps.
-		right. exists x1. 
-		eapply pc_trans in H;try exact Hunf.
-		eapply r_struct with (M2':=x1);try exact H;try easy.
-		constructor.
-
-		+ destr_hyps;subst.
-		assert(exists M2, betaP (x <-- (p_ite x1 x2 x3))  M2).
-		{
-		eapply inv_proc_ite in H1;try reflexivity;destr_hyps.
-		Search sbool.
-		eapply expr_eval_b in H4.
-		destruct H4.
-		eapply rt_iteu with (p:=x) (P:=x2) (Q:=x3) in H4; exists ((x <-- x2)); easy.      
-		
-		eapply rf_iteu with (p:=x) (P:=x2) (Q:=x3) in H4; exists ((x <-- x3)); easy.
-		}
-		destr_hyps.
-		right. exists x0. eapply pc_trans in H;try exact Hunf.
-		eapply r_struct with (M2':=x0);try exact H;try easy. constructor.
+		left; exists M'. split;tauto.
 	}
 	{
 		destruct Hdil as [p [q [xsp [xsq [Hfindp Hfindq]]]]].
@@ -494,9 +269,8 @@ Proof.
 		} 
 		assert(Hpq: p <> q) by (red;intros;subst;congruence).
 		eapply canonical_glob_nt in Hsess as Hcanon;try exact Hfindq;try exact Hfindp;try easy.
-		destruct Hcanon.
 		{
-			destruct H as [M' [P [Q Hunf]]].
+			destruct Hcanon as [M' [P [Q Hunf]]].
 			eapply typ_after_unfold in Hunf as Hsess';try exact Hsess.
 			inversion Hsess';subst. rename H1 into Hdup, H2 into Hfat. 
 			
@@ -506,81 +280,24 @@ Proof.
 			destr_hyps.
 			rewrite Hfindp in H1;inversion H1;subst;clear H1. 
 			rewrite Hfindq in H;inversion H;subst;clear H.
-			eapply guardP_break in H6 as Hgb. destruct Hgb as [P' [Hrec_unf Htr]].
-			Search typ_proc betaPr.
-			eapply typ_proc_after_betaPr in H5 as Htyp';try exact Hrec_unf.
+			eapply guardP_break_tau in H6 as Hgb;try exact H5. destruct Hgb as [P' [Hrec_unf Htr]].
+			eapply typ_after_tauRtc in H5 as Htyp';try exact Hrec_unf.
 			destruct Htr as [Htr | Htr];[| destruct Htr as [Htr | Htr]].
 			{
 				eapply inv_proc_inact in Htyp';try easy. 
 			}
 			{
-				destr_hyps;subst. eapply inv_proc_ite in Htyp';try reflexivity;destr_hyps.
-				set (Meq1 := (((p <-- (p_ite x x0 x1)) |||(q <-- Q )) ||| M')).
-				assert(Hunf' : unfoldP M Meq1).
-				{
-					assert(Hm:multi betaPr Q Q). constructor.
-					eauto with procs.					
-				}
-				set (Meq := (p <-- (p_ite x x0 x1)) |||((q <-- Q ) ||| M')).
-				assert(Hexp: unfoldP Meq Meq1) by eauto with procs.
-				assert(Hexp': unfoldP M Meq) by eauto with procs.
-
-				eapply expr_eval_b in H9;destruct H9.
-				assert (exists M'0, betaP Meq M'0).
-				{
-					unfold Meq.
-					exists (p <-- x0 ||| ((q <-- Q) ||| M')). eapply rt_ite;easy.
-				}
-				destr_hyps. exists x4. eapply r_struct with (M2':=x4);try exact Hexp';try easy;constructor.
-				
-				assert (exists M'0, betaP Meq M'0).
-				{
-					unfold Meq.
-					exists (p <-- x1 ||| ((q <-- Q) ||| M')). eapply rf_ite;easy.
-				}
-				destr_hyps. exists x4. eapply r_struct with (M2':=x4);try exact Hexp';try easy;constructor.
-			}
-			{
-				destruct Htr;destr_hyps;subst. 
-				{
+				destr_hyps;subst.
 				eapply inv_proc_send in Htyp';try reflexivity.
 				destr_hyps.
 				
-				eapply guardP_break in H4 as Htq. destruct Htq as [Q' [Hrec_unfq Htq]].
-				eapply typ_proc_after_betaPr in H2 as Htyq';try exact Hrec_unfq.
+				eapply guardP_break_tau in H4 as Htq;try exact H2. destruct Htq as [Q' [Hrec_unfq Htq]].
+				eapply typ_after_tauRtc in H2 as Htyq';try exact Hrec_unfq.
 
 				destruct Htq;subst. eapply inv_proc_inact in Htyq';try easy.
-				destruct H8. 
+				destruct H8; 
 				destr_hyps;subst.
-				{
-					eapply inv_proc_ite in Htyq';try reflexivity;destr_hyps.
-					set (Meq1 := (((q <-- (p_ite x5 x6 x7)) |||(p <-- P )) ||| M')).
-					assert(Hunf' : unfoldP M Meq1).
-					{
-						assert(Hm:multi betaPr P P). constructor.
-						eauto with procs.					
-					}
-					set (Meq := (q <-- (p_ite x5 x6 x7)) |||((p <-- P ) ||| M')).
-					assert(Hexp: unfoldP Meq Meq1) by eauto with procs.
-					assert(Hexp': unfoldP M Meq) by eauto with procs.
-
-					eapply expr_eval_b in H12;destruct H12.
-					assert (exists M'0, betaP Meq M'0).
-					{
-						unfold Meq.
-						exists (q <-- x6 ||| ((p <-- P) ||| M')). eapply rt_ite;easy.
-					}
-					destr_hyps. exists x10. eapply r_struct with (M2':=x10);try exact Hexp';try easy;constructor.
-					
-					assert (exists M'0, betaP Meq M'0).
-					{
-						unfold Meq.
-						exists (q <-- x7 ||| ((p <-- P) ||| M')). eapply rf_ite;easy.
-
-					}
-					destr_hyps. exists x10. eapply r_struct with (M2':=x10);try exact Hexp';try easy;constructor.
-				}
-				destruct H8. destr_hyps;subst.
+				
 				eapply inv_proc_send in Htyq';try reflexivity. destr_hyps.
 				pinversion H10;try apply sub_mon.
 				destr_hyps;subst.
@@ -616,472 +333,29 @@ Proof.
 				eapply subtype_recv_inv in H9. 
 				eapply Forall2R_prop in H9;try exact H16;tac_sanitize.
 				eapply Forall2_prop_l in H10;try exact H12;tac_sanitize.
-				assert(Hunf' : unfoldP M (((q <-- p_recv p chcs)) ||| (p <-- p_send q ell e P_c) ||| M')) by eauto with procs.
+				Search unfoldP tauRtc.
+				Check tauRtc_unfold.
+				Hint Resolve  tauRtc_unfold :procs.
+				assert(Hunf'' : unfoldP (((p <-- P) ||| (q <-- Q)) ||| M') (((p <-- p_send q ell e P_c) ||| (q <-- Q)) ||| M'))
+				by 
+				eauto with procs.
+
+				assert(Hunf' : unfoldP M (((q <-- p_recv p chcs)) ||| (p <-- p_send q ell e P_c) ||| M')) by  (eauto 7 with procs).
 				eapply expr_eval_ss in H;destr_hyps.
 				eapply r_comm with (p:=q) (q:=p) (e:=e) (Q:=P_c) (M:=M') (v:=x)  in H9 as Hbeta;try easy.
 				exists (((q <-- subst_expr_proc x6 (e_val x) 0 0) ||| (p <-- P_c)) ||| M').
 				eapply r_struct with (M2':= (((q <-- subst_expr_proc x6 (e_val x) 0 0)
 				||| (p <-- P_c)) ||| M'));try exact Hunf';try easy. constructor.
-				}
+			}
 				{
+					destr_hyps;subst.
 					eapply inv_proc_recv in Htyp';try reflexivity;subst;destr_hyps.
 					pinversion H1;subst;try apply sub_mon. 
 				}
 			}
 		}
-		(*without M'*)
-		{
-			destruct H as [P [Q Hunf]].
-			eapply typ_after_unfold in Hunf as Hsess';try exact Hsess.
-			inversion Hsess';subst. rename H1 into Hdup, H2 into Hfat. 
-			
-			clear Hassocable H.
-			inversion Hfat;subst. inversion_clear H2;subst. inversion_clear H3;subst.
-			destr_hyps.
-			rewrite Hfindp in H;inversion H;subst;clear H. 
-			rewrite Hfindq in H1;inversion H1;subst;clear H1.
-			eapply guardP_break in H5 as Hgb. destruct Hgb as [P' [Hrec_unf Htr]].
-			
-			eapply typ_proc_after_betaPr in H4 as Htyp';try exact Hrec_unf.
-			destruct Htr as [Htr | Htr];[| destruct Htr as [Htr | Htr]].
-			{
-				eapply inv_proc_inact in Htyp';try easy. 
-			}
-			{
-				destr_hyps;subst. eapply inv_proc_ite in Htyp';try reflexivity;destr_hyps.
-				set (Meq1 := (((p <-- (p_ite x x0 x1)) |||(q <-- Q )) )).
-				assert(Hunf' : unfoldP M Meq1).
-				{
-					assert(Hm:multi betaPr Q Q). constructor.
-					eauto with procs.					
-				}
-				set (Meq := (p <-- (p_ite x x0 x1)) |||((q <-- Q ) )).
-				assert(Hexp: unfoldP Meq Meq1) by eauto with procs.
-				assert(Hexp': unfoldP M Meq) by eauto with procs.
-
-				eapply expr_eval_b in H8;destruct H8.
-				assert (exists M'0, betaP Meq M'0).
-				{
-					unfold Meq.
-					exists (p <-- x0 ||| ((q <-- Q))). eapply rt_ite;easy.
-				}
-				destr_hyps. exists x4. eapply r_struct with (M2':=x4);try exact Hexp';try easy;constructor.
-				
-				assert (exists M'0, betaP Meq M'0).
-				{
-					unfold Meq.
-					exists (p <-- x1 ||| ((q <-- Q))). eapply rf_ite;easy.
-				}
-				destr_hyps. exists x4. eapply r_struct with (M2':=x4);try exact Hexp';try easy;constructor.
-			}
-			{
-				destruct Htr;destr_hyps;subst. 
-				{
-				eapply inv_proc_send in Htyp';try reflexivity.
-				destr_hyps.
-				
-				eapply guardP_break in H3 as Htq. destruct Htq as [Q' [Hrec_unfq Htq]].
-				eapply typ_proc_after_betaPr in H2 as Htyq';try exact Hrec_unfq.
-
-				destruct Htq;subst. eapply inv_proc_inact in Htyq';try easy.
-				destruct H7. 
-				destr_hyps;subst.
-				{
-					eapply inv_proc_ite in Htyq';try reflexivity;destr_hyps.
-					set (Meq1 := (((q <-- (p_ite x5 x6 x7)) |||(p <-- P )))).
-					assert(Hunf' : unfoldP M Meq1).
-					{
-						assert(Hm:multi betaPr P P). constructor.
-						eauto with procs.					
-					}
-					set (Meq := (q <-- (p_ite x5 x6 x7)) |||((p <-- P ))).
-					assert(Hexp: unfoldP Meq Meq1) by eauto with procs.
-					assert(Hexp': unfoldP M Meq) by eauto with procs.
-
-					eapply expr_eval_b in H11;destruct H11.
-					assert (exists M'0, betaP Meq M'0).
-					{
-						unfold Meq.
-						exists (q <-- x6 ||| ((p <-- P))). eapply rt_ite;easy.
-					}
-					destr_hyps. exists x10. eapply r_struct with (M2':=x10);try exact Hexp';try easy;constructor.
-					
-					assert (exists M'0, betaP Meq M'0).
-					{
-						unfold Meq.
-						exists (q <-- x7 ||| ((p <-- P))). eapply rf_ite;easy.
-
-					}
-					destr_hyps. exists x10. eapply r_struct with (M2':=x10);try exact Hexp';try easy;constructor.
-				}
-				destruct H7. destr_hyps;subst.
-				eapply inv_proc_send in Htyq';try reflexivity. destr_hyps.
-				pinversion H9;try apply sub_mon.
-				destr_hyps;subst.
-				
-				eapply inv_proc_recv in Htyq';try reflexivity. destr_hyps.
-				rename x into q', x0 into ell, x1 into e, x2 into P_c, x3 into se, x4 into Tpc.
-				rename x5 into p', x6 into chcs, x7 into xq'.
-				
-				assert (q'=q) by (pinversion H6;subst;try apply sub_mon;easy);subst.
-				assert (p'=p) by (pinversion H8;subst;try apply sub_mon;easy);subst.
-				
-				assert (Hsubq: assoc.issubProj (ltt_recv p xsq) g q) by
-					(eapply assoc_inv_find with (g:=g) in Hfindq; easy).
-				
-				assert (Hsubp: assoc.issubProj (ltt_send q xsp) g p) by 
-				(eapply assoc_inv_find with (g:=g) in Hfindp; easy).
-				assert (Hax1 : SList xsp) by
-					(specialize (Htwf _ _ Hfindp); pinversion Htwf;subst;try apply wfltt.wfltt_mon;easy).
-				
-				assert (Hax2 : SList xsq) by
-					(specialize (Htwf _ _ Hfindq); pinversion Htwf;subst;try apply wfltt.wfltt_mon;easy).
-				assert(Hispartsp: isgPartsC p g).
-				{
-					destruct (decidable.decidable_isgPartsC g p);try easy.
-					red in Hsubp;destr_hyps. eapply assoc.subtype_send_inv1 in H13. destr_hyps;subst.
-					pinversion H12;subst;try easy;try apply proj_mon.
-				}
-				eapply assoc.lem_6_16_simul_subproj in Hsubp as Hsimul;try exact Hsubq;try easy.
-				move H6 at bottom. eapply subtype_send_inv in H6.
-				assert(Honthl: onth ell (extendLis ell (Some (se, Tpc)))=Some (se,Tpc)) by (rewrite extendExtract;easy).
-				eapply Forall2R_prop in H6;try exact Honthl;tac_sanitize.
-				eapply Forall2R_prop in Hsimul;try exact H12;tac_sanitize.
-				eapply subtype_recv_inv in H8. 
-				eapply Forall2R_prop in H8;try exact H15;tac_sanitize.
-				eapply Forall2_prop_l in H9;try exact H11;tac_sanitize.
-				assert(Hunf' : unfoldP M (((q <-- p_recv p chcs)) ||| (p <-- p_send q ell e P_c))) by eauto with procs.
-				eapply expr_eval_ss in H;destr_hyps.
-				Print betaP.
-				eapply r_commu with (p:=q) (q:=p) (e:=e) (Q:=P_c) (v:=x)  in H8 as Hbeta;try easy.
-				exists (((q <-- subst_expr_proc x6 (e_val x) 0 0) ||| (p <-- P_c))).
-				eapply r_struct with (M2':= (((q <-- subst_expr_proc x6 (e_val x) 0 0)
-				||| (p <-- P_c))));try exact Hunf';try easy. constructor.
-				}
-				{
-					eapply inv_proc_recv in Htyp';try reflexivity;subst;destr_hyps.
-					pinversion H1;subst;try apply sub_mon. 
-				}
-			}
-		}
-	}
 Qed.
 
-Theorem prog : forall M G, typ_sess M G -> (exists M', unfoldP M M' /\ (ForallT (fun _ P => P = p_inact) M')) \/ exists M', betaP M M'.
-Proof.
-  intros.
-  destruct G.
-  - specialize(canonical_glob_n M H); intros.
-    destruct H0 as (M',(Ha,Hb)).
-    assert(ForallT (fun _ P => P = p_inact) M' \/ (exists p e p1 p2, typ_proc nil nil (p_ite e p1 p2) ltt_end /\ ((exists M'', unfoldP M' ((p <-- p_ite e p1 p2) ||| M'')) \/ unfoldP M' (p <-- p_ite e p1 p2)))).
-    {
-      clear H Ha. clear M. revert Hb.
-      induction M'; intros.
-      - inversion Hb. subst. clear Hb. destruct H0.
-        - subst. left. constructor. easy.
-        - destruct H as (e,(p1,(p2,(Ha,Hb)))).
-          right. exists n. exists e. exists p1. exists p2.  
-          split. easy.
-          right. subst. apply pc_refl.
-      - inversion Hb. subst. clear Hb.
-        specialize(IHM'1 H1). specialize(IHM'2 H2). clear H1 H2.
-        destruct IHM'1.
-        - destruct IHM'2. left. constructor; try easy.
-        - destruct H0 as (p0,(e,(p1,(p2,(Ha,Hb))))).
-          right. exists p0. exists e. exists p1. exists p2. split. easy.
-          left. destruct Hb.
-          - destruct H0 as (M1,Hc).
-            exists (M1 ||| M'1).
-            apply pc_trans with (M' := M'2 ||| M'1). constructor.
-            apply pc_trans with (M' := ((p0 <-- p_ite e p1 p2) ||| M1) ||| M'1).
-            apply unf_cont_l. easy. constructor.
-          - exists M'1. 
-            apply pc_trans with (M' := M'2 ||| M'1). constructor.
-            apply unf_cont_l. easy.
-        - destruct H as (p,(e,(p1,(p2,(Ha,Hb))))).
-          destruct Hb.
-          - destruct H as (M',H). 
-            right. exists p. exists e. exists p1. exists p2. split. easy.
-            left. exists (M' ||| M'2).
-            apply pc_trans with (M' := ((p <-- p_ite e p1 p2 ||| M') ||| M'2)). apply unf_cont_l. easy.
-            constructor.
-          - right. exists p. exists e. exists p1. exists p2.
-            split. easy.
-            left. exists M'2. apply unf_cont_l. easy.
-    }
-    clear Hb. destruct H0.
-    - left. exists M'. easy.
-    - destruct H0 as (p,(e,(p1,(p2,(Hb,Hc))))). right.
-      destruct Hc. 
-      - destruct H0 as (M1,H0).
-        assert(unfoldP M ((p <-- p_ite e p1 p2) ||| M1)). apply pc_trans with (M' := M'); try easy.
-        clear H0 Ha.
-        assert(exists M2, betaP ((p <-- p_ite e p1 p2) ||| M1) M2).
-        {
-          specialize(inv_proc_ite (p_ite e p1 p2) e p1 p2 ltt_end nil nil Hb (erefl (p_ite e p1 p2))); intros.
-          destruct H0 as (T1,(T2,(Ha,(Hf,(Hc,(Hd,He)))))).
-          specialize(expr_eval_b e He); intros.
-          destruct H0.
-          - exists ((p <-- p1) ||| M1). constructor. easy.
-          - exists ((p <-- p2) ||| M1). constructor. easy.
-        }
-        destruct H0 as (M2,H0). exists M2.
-        apply r_struct with (M1' := ((p <-- p_ite e p1 p2) ||| M1)) (M2' := M2); try easy. 
-        constructor.
-      - assert(exists M2, betaP ((p <-- p_ite e p1 p2)) M2).
-        { 
-          specialize(inv_proc_ite (p_ite e p1 p2) e p1 p2 ltt_end nil nil Hb (erefl (p_ite e p1 p2))); intros.
-          destruct H1 as (T1,(T2,(Hg,(Hf,(Hc,(Hd,He)))))).
-          specialize(expr_eval_b e He); intros. destruct H1.
-          - exists ((p <-- p1)). constructor. easy.
-          - exists ((p <-- p2)). constructor. easy.
-        }
-        destruct H1 as (M2,H1). exists M2.
-        apply r_struct with (M1' := (p <-- p_ite e p1 p2)) (M2' := M2); try easy.
-        apply pc_trans with (M' := M'); try easy. constructor.
-  - right.
-    rename n into p. rename n0 into q.
-    specialize(canonical_glob_nt M p q l H); intros.
-    destruct H0.
-    - destruct H0 as (M',(P,(Q,Ha))).
-      specialize(typ_after_unfold M (((p <-- P) ||| (q <-- Q)) ||| M') (gtt_send p q l)); intros.
-      assert(typ_sess (((p <-- P) ||| (q <-- Q)) ||| M') (gtt_send p q l)). apply H0; try easy.
-      clear H0.
-      assert(exists M1, betaP (((p <-- P) ||| (q <-- Q)) ||| M') M1).
-      {
-        inversion H1. subst. inversion H4. subst. clear H4. inversion H7. subst. clear H7.
-        inversion H6. subst. clear H6. inversion H9. subst. clear H9.
-        destruct H5 as (T,(Hd,(Hb,Hc))). destruct H6 as (T1,(He,(Hf,Hg))).
-        clear Ha H2 H3 H8.
-        specialize(guardP_break P Hc); intros.
-        destruct H2 as (Q1,(Hh,Ho)).
-        specialize(typ_proc_after_betaPr P Q1 nil nil T Hh Hb); intros.
-        pinversion Hd. subst. assert False. apply H3. apply triv_pt_p; try easy. easy. subst. easy. subst. 
-        - specialize(guardP_break Q Hg); intros.
-          destruct H3 as (Q2,(Hj,Hl)).
-          specialize(typ_proc_after_betaPr Q Q2 nil nil T1 Hj Hf); intros.
-          clear H7 H9 Hg Hc H H1 Hd.
-          pinversion He; try easy. subst. assert False. apply H. apply triv_pt_q; try easy. easy.
-          subst. clear H7 H9 H5 He Hb Hf.
-          assert(exists M1, betaP (((p <-- Q1) ||| (q <-- Q2)) ||| M') M1).
-          {
-            clear Hh Hj.
-            destruct Ho.
-            - subst. specialize(inv_proc_inact p_inact (ltt_send q ys) nil nil H2 (erefl (p_inact))); intros. 
-              easy.
-            - destruct H. destruct H as (e,(p1,(p2,Ha))). subst.
-              specialize(inv_proc_ite (p_ite e p1 p2) e p1 p2 (ltt_send q ys) nil nil H2 (erefl (p_ite e p1 p2))); intros.
-              destruct H as (T1,(T2,(Ha,(Hb,(Hc,(Hd,He)))))).
-              specialize(expr_eval_b e He); intros. 
-              destruct H.
-              - exists ((p <-- p1) ||| ((q <-- Q2) ||| M')).
-                apply r_struct with (M1' := ((p <-- p_ite e p1 p2) ||| ((q <-- Q2) ||| M'))) (M2' := ((p <-- p1) ||| ((q <-- Q2) ||| M'))); try easy. constructor. constructor. constructor. easy.
-              - exists ((p <-- p2) ||| ((q <-- Q2) ||| M')).
-                apply r_struct with (M1' := ((p <-- p_ite e p1 p2) ||| ((q <-- Q2) ||| M'))) (M2' := ((p <-- p2) ||| ((q <-- Q2) ||| M'))); try easy. constructor. constructor. constructor. easy.
-            - destruct H.
-              destruct H as (pt,(lb,(ex,(pr,Ha)))). subst.
-              specialize(inv_proc_send pt lb ex pr (p_send pt lb ex pr) nil nil (ltt_send q ys) H2 (erefl ((p_send pt lb ex pr)))); intros. destruct H as (S,(T1,(Ht,Hb))). clear H2. rename T1 into Tl. rename Hb into Hta. clear M P Q.
-              destruct Hl.
-              - subst. specialize(inv_proc_inact p_inact (ltt_recv p ys0) nil nil H3 (erefl (p_inact))); intros. 
-                easy.
-              - destruct H. destruct H as (e,(p1,(p2,Ha))). subst. 
-                specialize(inv_proc_ite (p_ite e p1 p2) e p1 p2 (ltt_recv p ys0) nil nil H3 (erefl (p_ite e p1 p2))); intros.
-                destruct H as (T1,(T2,(Ha,(Hb,(Hc,(Hd,He)))))).
-                specialize(expr_eval_b e He); intros. 
-                destruct H.
-                - exists ((q <-- p1) ||| ((p <-- p_send pt lb ex pr) ||| M')).
-                  apply r_struct with (M1' := ((q <-- p_ite e p1 p2) ||| ((p <-- p_send pt lb ex pr) ||| M'))) (M2' := ((q <-- p1) ||| ((p <-- p_send pt lb ex pr) ||| M'))).
-                  apply pc_trans with (M' := ((q <-- p_ite e p1 p2) ||| (p <-- p_send pt lb ex pr)) ||| M').
-                  constructor. constructor. apply unf_cont_r. constructor.
-                  constructor. easy.
-                - exists ((q <-- p2) ||| ((p <-- p_send pt lb ex pr) ||| M')).
-                  apply r_struct with (M1' := ((q <-- p_ite e p1 p2) ||| ((p <-- p_send pt lb ex pr) ||| M'))) (M2' := ((q <-- p2) ||| ((p <-- p_send pt lb ex pr) ||| M'))).
-                  apply pc_trans with (M' := ((q <-- p_ite e p1 p2) ||| (p <-- p_send pt lb ex pr)) ||| M').
-                  constructor. constructor. apply unf_cont_r. constructor.
-                  constructor. easy.
-              - destruct H. destruct H as (pt1,(lb1,(ex1,(pr1,Ha)))). subst.
-                specialize(inv_proc_send pt1 lb1 ex1 pr1 (p_send pt1 lb1 ex1 pr1) nil nil (ltt_recv p ys0) H3 (erefl (p_send pt1 lb1 ex1 pr1))); intros.
-                destruct H as (S1,(T1,(Ha,(Hb,Hc)))). pinversion Hc. apply sub_mon.
-              - destruct H as (pt2,(llp,Ha)). subst.
-                specialize(expr_eval_ss ex S Ht); intros. destruct H as (v, Ha).
-                destruct Hta as (Hta,Htb).
-                pinversion Htb. subst.
-                specialize(inv_proc_recv pt2 llp (p_recv pt2 llp) nil nil (ltt_recv p ys0) H3 (erefl (p_recv pt2 llp))); intros.
-                destruct H as (STT,(He,(Hb,(Hc,Hd)))).
-                pinversion Hb. subst.
-                assert(exists y, onth lb llp = Some y).
-                {
-                  specialize(subtype_send_inv q (extendLis lb (Some (S, Tl))) ys); intros.
-                  assert(Forall2R
-                    (fun u v : option (sort * ltt) =>
-                     u = None \/
-                     (exists (s s' : sort) (t t' : ltt),
-                        u = Some (s, t) /\ v = Some (s', t') /\ subsort s s' /\ subtypeC t t'))
-                    (extendLis lb (Some (S, Tl))) ys). apply H; try easy.
-                  pfold. easy.
-                  
-                  specialize(subtype_recv_inv p STT ys0); intros.
-                  assert(Forall2R
-                   (fun u v : option (sort * ltt) =>
-                    u = None \/
-                    (exists (s s' : sort) (t t' : ltt),
-                       u = Some (s, t) /\ v = Some (s', t') /\ subsort s s' /\ subtypeC t' t)) ys0 STT). apply H5. pfold. easy.
-                  clear H2 H5 Hd Hb He H H1 Ha Htb Hta Ht H3 H6 H0.
-                  revert H7 Hc H4 H11 H10.
-                  revert p q l ys ys0 llp S Tl STT. 
-                  induction lb; intros.
-                  - destruct ys; try easy. destruct l; try easy. destruct ys0; try easy. destruct STT; try easy. destruct llp; try easy.
-                    inversion H10. subst. clear H10. inversion H11. subst. clear H11. inversion H7. subst. clear H7. inversion Hc. subst. clear Hc. inversion H4. subst. clear H4.
-                    clear H13 H11 H10 H8 H5.
-                    destruct H9; try easy. destruct H as (s1,(s2,(t1,(t2,(Ha,(Hb,(Hc,Hd))))))). subst.
-                    destruct H2; try easy. destruct H as (s3,(g1,(t3,(He,(Hf,Hg))))). subst.
-                    destruct H3; try easy. destruct H as (s4,(g2,(t4,(Hh,(Hi,Hj))))). subst.
-                    destruct H6; try easy. destruct H as (s5,(s6,(t5,(t6,(Hk,(Hl,(Hm,Hn))))))). subst.
-                    destruct H7; try easy. destruct H as (p1,(s7,(t7,(Ho,(Hp,Hq))))). subst.
-                    exists p1. easy.
-                  - destruct ys; try easy. destruct l; try easy. destruct ys0; try easy. destruct STT; try easy. destruct llp; try easy.
-                    inversion H10. subst. clear H10. inversion H11. subst. clear H11. inversion H7. subst. clear H7. inversion Hc. subst. clear Hc. inversion H4. subst. clear H4.
-                    specialize(IHlb p q l ys ys0 llp S Tl STT). apply IHlb; try easy.
-                }
-                destruct H as (y, H).
-                exists ((q <-- subst_expr_proc y (e_val v) 0 0) ||| (p <-- pr) ||| M').
-                apply r_struct with (M1' := (((q <-- p_recv p llp) ||| (p <-- p_send q lb ex pr)) ||| M')) (M2' := (((q <-- subst_expr_proc y (e_val v) 0 0) ||| (p <-- pr)) ||| M')); try easy.
-                constructor. constructor. constructor. easy. easy.
-                apply sub_mon. apply sub_mon.
-            - destruct H as (pt,(llp,Ha)). subst.
-              specialize(inv_proc_recv pt llp (p_recv pt llp) nil nil (ltt_send q ys) H2 (erefl (p_recv pt llp))); intros.
-              destruct H as (STT,(Ha,(Hb,Hc))). pinversion Hb. apply sub_mon.
-          }
-          destruct H as (M1,Hta). exists M1.
-          apply r_struct with (M1' := (((p <-- Q1) ||| (q <-- Q2)) ||| M')) (M2' := M1); try easy.
-          apply betaPr_unfold; try easy.
-          constructor.
-          apply proj_mon.
-        subst. easy.
-        apply proj_mon.
-      }
-      destruct H0 as (M1,H0). exists M1.
-      apply r_struct with (M1' := (((p <-- P) ||| (q <-- Q)) ||| M')) (M2' := M1); try easy. constructor.
-    - destruct H0 as (P,(Q,Ha)).
-      specialize(typ_after_unfold M (((p <-- P) ||| (q <-- Q))) (gtt_send p q l)); intros.
-      assert(typ_sess ((p <-- P) ||| (q <-- Q)) (gtt_send p q l)). apply H0; try easy.
-      clear H0.
-      assert(exists M1, betaP (((p <-- P) ||| (q <-- Q))) M1).
-      {
-        inversion H1. subst. inversion H4. subst. clear H4. inversion H7. subst. clear H7.
-        inversion H8. subst. clear H8.
-        destruct H5 as (T,(Hd,(Hb,Hc))). destruct H6 as (T1,(He,(Hf,Hg))).
-        clear Ha H2 H3.
-        specialize(guardP_break P Hc); intros.
-        destruct H2 as (Q1,(Hh,Ho)).
-        specialize(typ_proc_after_betaPr P Q1 nil nil T Hh Hb); intros.
-        pinversion Hd. subst. assert False. apply H3. apply triv_pt_p; try easy. easy. subst. easy. subst. 
-        - specialize(guardP_break Q Hg); intros.
-          destruct H3 as (Q2,(Hj,Hl)).
-          specialize(typ_proc_after_betaPr Q Q2 nil nil T1 Hj Hf); intros.
-          clear H7 H9 Hg Hc H H1 Hd.
-          pinversion He; try easy. subst. assert False. apply H. apply triv_pt_q; try easy. easy.
-          subst. clear H7 H9 H5 He Hb Hf.
-          assert(exists M1, betaP (((p <-- Q1) ||| (q <-- Q2))) M1).
-          {
-            clear Hh Hj.
-            destruct Ho.
-            - subst. specialize(inv_proc_inact p_inact (ltt_send q ys) nil nil H2 (erefl (p_inact))); intros. 
-              easy.
-            - destruct H. destruct H as (e,(p1,(p2,Ha))). subst.
-              specialize(inv_proc_ite (p_ite e p1 p2) e p1 p2 (ltt_send q ys) nil nil H2 (erefl (p_ite e p1 p2))); intros.
-              destruct H as (T1,(T2,(Ha,(Hb,(Hc,(Hd,He)))))).
-              specialize(expr_eval_b e He); intros. 
-              destruct H.
-              - exists ((p <-- p1) ||| ((q <-- Q2))).
-                apply r_struct with (M1' := ((p <-- p_ite e p1 p2) ||| ((q <-- Q2)))) (M2' := ((p <-- p1) ||| ((q <-- Q2)))); try easy. constructor. constructor. constructor. easy.
-              - exists ((p <-- p2) ||| ((q <-- Q2))).
-                apply r_struct with (M1' := ((p <-- p_ite e p1 p2) ||| ((q <-- Q2)))) (M2' := ((p <-- p2) ||| ((q <-- Q2)))); try easy. constructor. constructor. constructor. easy.
-            - destruct H.
-              destruct H as (pt,(lb,(ex,(pr,Ha)))). subst.
-              specialize(inv_proc_send pt lb ex pr (p_send pt lb ex pr) nil nil (ltt_send q ys) H2 (erefl ((p_send pt lb ex pr)))); intros. destruct H as (S,(T1,(Ht,Hb))). clear H2. rename T1 into Tl. rename Hb into Hta. clear M P Q.
-              destruct Hl.
-              - subst. specialize(inv_proc_inact p_inact (ltt_recv p ys0) nil nil H3 (erefl (p_inact))); intros. 
-                easy.
-              - destruct H. destruct H as (e,(p1,(p2,Ha))). subst. 
-                specialize(inv_proc_ite (p_ite e p1 p2) e p1 p2 (ltt_recv p ys0) nil nil H3 (erefl (p_ite e p1 p2))); intros.
-                destruct H as (T1,(T2,(Ha,(Hb,(Hc,(Hd,He)))))).
-                specialize(expr_eval_b e He); intros. 
-                destruct H.
-                - exists ((q <-- p1) ||| ((p <-- p_send pt lb ex pr))).
-                  apply r_struct with (M1' := ((q <-- p_ite e p1 p2) ||| ((p <-- p_send pt lb ex pr)))) (M2' := ((q <-- p1) ||| ((p <-- p_send pt lb ex pr)))).
-                  apply pc_trans with (M' := ((q <-- p_ite e p1 p2) ||| (p <-- p_send pt lb ex pr))).
-                  constructor. constructor. apply unf_cont_r. constructor.
-                  constructor. easy.
-                - exists ((q <-- p2) ||| ((p <-- p_send pt lb ex pr))).
-                  apply r_struct with (M1' := ((q <-- p_ite e p1 p2) ||| ((p <-- p_send pt lb ex pr)))) (M2' := ((q <-- p2) ||| ((p <-- p_send pt lb ex pr)))).
-                  apply pc_trans with (M' := ((q <-- p_ite e p1 p2) ||| (p <-- p_send pt lb ex pr))).
-                  constructor. constructor. apply unf_cont_r. constructor.
-                  constructor. easy.
-              - destruct H. destruct H as (pt1,(lb1,(ex1,(pr1,Ha)))). subst.
-                specialize(inv_proc_send pt1 lb1 ex1 pr1 (p_send pt1 lb1 ex1 pr1) nil nil (ltt_recv p ys0) H3 (erefl (p_send pt1 lb1 ex1 pr1))); intros.
-                destruct H as (S1,(T1,(Ha,(Hb,Hc)))). pinversion Hc. apply sub_mon.
-              - destruct H as (pt2,(llp,Ha)). subst.
-                specialize(expr_eval_ss ex S Ht); intros. destruct H as (v, Ha).
-                destruct Hta as (Hta,Htb).
-                pinversion Htb. subst.
-                specialize(inv_proc_recv pt2 llp (p_recv pt2 llp) nil nil (ltt_recv p ys0) H3 (erefl (p_recv pt2 llp))); intros.
-                destruct H as (STT,(He,(Hb,(Hc,Hd)))).
-                pinversion Hb. subst.
-                assert(exists y, onth lb llp = Some y).
-                {
-                  specialize(subtype_send_inv q (extendLis lb (Some (S, Tl))) ys); intros.
-                  assert(Forall2R
-                    (fun u v : option (sort * ltt) =>
-                     u = None \/
-                     (exists (s s' : sort) (t t' : ltt),
-                        u = Some (s, t) /\ v = Some (s', t') /\ subsort s s' /\ subtypeC t t'))
-                    (extendLis lb (Some (S, Tl))) ys). apply H; try easy.
-                  pfold. easy.
-                  
-                  specialize(subtype_recv_inv p STT ys0); intros.
-                  assert(Forall2R
-                   (fun u v : option (sort * ltt) =>
-                    u = None \/
-                    (exists (s s' : sort) (t t' : ltt),
-                       u = Some (s, t) /\ v = Some (s', t') /\ subsort s s' /\ subtypeC t' t)) ys0 STT). apply H5. pfold. easy.
-                  clear H2 H5 Hd Hb He H H1 Ha Htb Hta Ht H3 H6 H0.
-                  revert H7 Hc H4 H11 H10.
-                  revert p q l ys ys0 llp S Tl STT. 
-                  induction lb; intros.
-                  - destruct ys; try easy. destruct l; try easy. destruct ys0; try easy. destruct STT; try easy. destruct llp; try easy.
-                    inversion H10. subst. clear H10. inversion H11. subst. clear H11. inversion H7. subst. clear H7. inversion Hc. subst. clear Hc. inversion H4. subst. clear H4.
-                    clear H13 H11 H10 H8 H5.
-                    destruct H9; try easy. destruct H as (s1,(s2,(t1,(t2,(Ha,(Hb,(Hc,Hd))))))). subst.
-                    destruct H2; try easy. destruct H as (s3,(g1,(t3,(He,(Hf,Hg))))). subst.
-                    destruct H3; try easy. destruct H as (s4,(g2,(t4,(Hh,(Hi,Hj))))). subst.
-                    destruct H6; try easy. destruct H as (s5,(s6,(t5,(t6,(Hk,(Hl,(Hm,Hn))))))). subst.
-                    destruct H7; try easy. destruct H as (p1,(s7,(t7,(Ho,(Hp,Hq))))). subst.
-                    exists p1. easy.
-                  - destruct ys; try easy. destruct l; try easy. destruct ys0; try easy. destruct STT; try easy. destruct llp; try easy.
-                    inversion H10. subst. clear H10. inversion H11. subst. clear H11. inversion H7. subst. clear H7. inversion Hc. subst. clear Hc. inversion H4. subst. clear H4.
-                    specialize(IHlb p q l ys ys0 llp S Tl STT). apply IHlb; try easy.
-                }
-                destruct H as (y, H).
-                exists ((q <-- subst_expr_proc y (e_val v) 0 0) ||| (p <-- pr)).
-                apply r_struct with (M1' := (((q <-- p_recv p llp) ||| (p <-- p_send q lb ex pr)))) (M2' := (((q <-- subst_expr_proc y (e_val v) 0 0) ||| (p <-- pr)))); try easy.
-                constructor. constructor. constructor. easy. easy.
-                apply sub_mon. apply sub_mon.
-            - destruct H as (pt,(llp,Ha)). subst.
-              specialize(inv_proc_recv pt llp (p_recv pt llp) nil nil (ltt_send q ys) H2 (erefl (p_recv pt llp))); intros.
-              destruct H as (STT,(Ha,(Hb,Hc))). pinversion Hb. apply sub_mon.
-          }
-          destruct H as (M1,Hta). exists M1.
-          apply r_struct with (M1' := (((p <-- Q1) ||| (q <-- Q2)))) (M2' := M1); try easy.
-          apply betaPr_unfold_h; try easy.
-          constructor.
-          apply proj_mon.
-        subst. easy.
-        apply proj_mon.
-      }
-      destruct H0 as (M1,H0). exists M1.
-      apply r_struct with (M1' := (((p <-- P) ||| (q <-- Q)))) (M2' := M1); try easy. constructor.
-Qed.
 
 
 Theorem stuck_free : forall M G, typ_sess M G -> stuckM M -> False.
